code/experimental/rsa/Hacl.RSAPSS.fst
@@ -16,9 +16,10 @@ val rsa_pss_sign:
     pow2_i:size_t -> iLen:size_t ->
     modBits:size_t{0 < v modBits /\ v modBits + 3 < max_size_t} ->
     eBits:size_t{0 < v eBits /\ v eBits <= v modBits} ->
-    dBits:size_t{0 < v dBits /\ v dBits <= v modBits /\
-		 v (bits_to_bn modBits) + v (bits_to_bn eBits) + v (bits_to_bn dBits) < max_size_t} ->
-    skey:lbignum (v (bits_to_bn modBits) + v (bits_to_bn eBits) + v (bits_to_bn dBits)) ->
+    dBits:size_t{0 < v dBits /\ v dBits <= v modBits} ->
+    pLen:size_t -> qLen:size_t{v (bits_to_bn modBits) + v (bits_to_bn eBits) + v (bits_to_bn dBits) + v pLen + v qLen < max_size_t} ->
+    skey:lbignum (v (bits_to_bn modBits) + v (bits_to_bn eBits) + v (bits_to_bn dBits) + v pLen + v qLen) ->
+    rBlind:uint64 ->
     ssLen:size_t{v ssLen == sLen /\ sLen + v hLen + 8 < max_size_t /\ v (blocks modBits (size 8)) - sLen - v hLen - 3 >= 0 } ->
     salt:lbytes sLen ->
     mmsgLen:size_t{v mmsgLen == msgLen /\ msgLen < pow2 61} -> msg:lbytes msgLen ->
@@ -27,8 +28,8 @@ val rsa_pss_sign:
 	              disjoint msg salt /\ disjoint msg sgnt /\ disjoint sgnt salt))
     (ensures (fun h0 _ h1 -> preserves_live h0 h1 /\ modifies1 sgnt h0 h1))
 
-let rsa_pss_sign #sLen #msgLen pow2_i iLen modBits eBits dBits skey ssLen salt mmsgLen msg sgnt = 
-    Hacl.Impl.RSA.rsa_sign #sLen #msgLen pow2_i iLen modBits eBits dBits skey ssLen salt mmsgLen msg sgnt
+let rsa_pss_sign #sLen #msgLen pow2_i iLen modBits eBits dBits pLen qLen skey rBlind ssLen salt mmsgLen msg sgnt =
+    Hacl.Impl.RSA.rsa_sign #sLen #msgLen pow2_i iLen modBits eBits dBits pLen qLen skey rBlind ssLen salt mmsgLen msg sgnt
 
 val rsa_pss_verify:
     #sLen:size_nat -> #msgLen:size_nat ->
@@ -43,5 +44,5 @@ val rsa_pss_verify:
     (requires (fun h -> live h msg /\ live h sgnt /\ live h pkey /\ disjoint msg sgnt))
     (ensures (fun h0 _ h1 -> preserves_live h0 h1 /\ modifies0 h0 h1))
 
-let rsa_pss_verify #sLen #msgLen pow2_i iLen modBits eBits pkey ssLen sgnt mmsgLen msg = 
+let rsa_pss_verify #sLen #msgLen pow2_i iLen modBits eBits pkey ssLen sgnt mmsgLen msg =
     Hacl.Impl.RSA.rsa_verify #sLen #msgLen pow2_i iLen modBits eBits pkey ssLen sgnt mmsgLen msg
